theories/LambdaCube/Typing.v
@@ -90,7 +90,7 @@ Definition system_omega : pi_scheme :=
 Definition systemPF : pi_scheme :=
   fun s s' => is_star s || is_star s'.
 
-Notation "'PF'" := systemP.
+Notation "'PF'" := systemPF.
 
 Definition P_weak_omega : pi_scheme :=
   fun s s' => is_star s || is_box s'.
@@ -101,3 +101,259 @@ Definition CoC : pi_scheme :=
   fun s s' => true.
 
 Notation "'C'" := CoC.
+
+Lemma typ_star_inv Sc {n} (Γ : typing_ctx n) t : Γ ⊢(Sc) Srt Star : t -> t ≅ Srt Box.
+Proof.
+  remember (Srt Star). induction 1; try discriminate; try solve [constructor].
+  intuition subst. eapply Requiv_trans; try eassumption. apply Requiv_sym. assumption.
+Qed.
+
+Lemma typ_var_inv Sc {n} (Γ : typing_ctx n) i T :
+  (Γ ⊢(Sc) Var i : T) -> T ≅ kth_index_ctx Γ (proj1_sig i) (proj2_sig i).
+  remember (Var i). induction 1 in i, Heqt |- *; try discriminate.
+  - inversion Heqt. subst. constructor.
+  - subst. specialize (IHtyping _ eq_refl). eapply Requiv_trans; eauto using Requiv_sym.
+Qed.
+
+Lemma typ_pi_inv Sc {n} (Γ : typing_ctx n) A B T :
+  Γ ⊢(Sc) Pi A B : T -> exists s s',
+        T ≅ Srt s' /\ Γ ⊢(Sc) A : Srt s /\ Γ, A ⊢(Sc) B : Srt s' /\ pi_scheme_check Sc s s'.
+Proof.
+  remember (Pi A B). induction 1 in A, B, Heqt |- *; try discriminate.
+  - exists s. exists s'. inversion Heqt; subst; clear Heqt. intuition constructor.
+  - subst. specialize (IHtyping _ _ eq_refl). destruct IHtyping as [s [s']].
+    exists s. exists s'. intuition. eauto using Requiv_trans, Requiv_sym.
+Qed.
+
+Lemma typ_abs_inv Sc {n} (Γ: typing_ctx n) A t T :
+  Γ ⊢(Sc) Abs A t : T ->
+  exists s s' B,
+    T ≅ Pi A B /\ Γ ⊢(Sc) A : Srt s /\ Γ, A ⊢(Sc) B : Srt s' /\ Γ, A ⊢(Sc) t : B /\
+      pi_scheme_check Sc s s'.
+Proof.
+  remember (Abs A t).
+  induction 1 in A, t, Heqt0 |- *; try discriminate.
+  - clear IHtyping1 IHtyping2 IHtyping3. inversion Heqt0. subst. clear Heqt0.
+    exists s. exists s'. exists B. intuition constructor.
+  - subst. specialize (IHtyping A t eq_refl).
+    destruct IHtyping as [s [s' [B0]]].
+    exists s. exists s'. exists B0. intuition eauto using Requiv_trans, Requiv_sym.
+Qed.
+
+Lemma typ_app_inv Sc {n} (Γ: typing_ctx n) t u T :
+  Γ ⊢(Sc) App t u : T -> exists A B, T ≅ bind (bind_first u) B /\ Γ ⊢(Sc) t : Pi A B /\ Γ ⊢(Sc) u : A.
+Proof.
+  remember (App t u) as t0.
+  induction 1 in t, u, Heqt0 |- *; try discriminate.
+  - clear IHtyping1 IHtyping2. exists A, B. inversion Heqt0; subst; clear Heqt0. intuition constructor.
+  - subst. specialize (IHtyping _ _ eq_refl).
+    destruct IHtyping as [A0 [B0]].
+    exists A0, B0. intuition eauto using Requiv_trans, Requiv_sym.
+Qed.
+
+Lemma typing_imp_ctx_wf Sc {n} (Γ: typing_ctx n) t s : Γ ⊢(Sc) t : s -> Γ ⊢(Sc).
+Proof.
+  induction 1; try assumption.
+Qed.
+
+Lemma equiv_context (Sc : pi_scheme) {n} (Γ Γ': typing_ctx n) t s :
+  (forall k H, kth_index_ctx Γ' k H ≅ kth_index_ctx Γ k H) -> Γ' ⊢(Sc) -> Γ ⊢(Sc) t : s -> Γ' ⊢(Sc) t : s.
+Proof.
+  intros H pr. induction 1.
+  - constructor. assumption.
+  - econstructor; swap 1 2. { apply H. } constructor. assumption.
+  - econstructor; try eassumption; auto.
+    apply IHtyping2.
+    + intros. simpl. destruct (lt_dec k n); try solve [constructor].
+      apply ren_preserves_step_equiv. auto.
+    + econstructor; try eassumption.
+      apply IHtyping1; assumption.
+  - econstructor; try eassumption; auto.
+    + apply IHtyping2.
+      * intros. simpl. destruct (lt_dec k n); try solve [constructor].
+        apply ren_preserves_step_equiv. auto.
+      * econstructor; try eassumption.
+        apply IHtyping1; assumption.
+    + apply IHtyping3.
+      * intros. simpl. destruct (lt_dec k n); try solve [constructor].
+        apply ren_preserves_step_equiv. auto.
+      * econstructor; try assumption. apply IHtyping1; assumption.
+  - econstructor; auto.
+  - econstructor; eauto.
+Qed.
+
+Lemma weakening {Sc n k} {σ: {i | i < n} -> {i | i < k}} {Γ Γ' x T}  :
+  (forall i,
+      ren σ (kth_index_ctx Γ (proj1_sig i) (proj2_sig i)) =
+        kth_index_ctx Γ' (proj1_sig (σ i)) (proj2_sig (σ i))) ->
+  Γ ⊢(Sc) x : T -> Γ' ⊢(Sc) -> Γ' ⊢(Sc) ren σ x : ren σ T.
+  intro H. induction 1 in k, σ, Γ', H |- *; simpl; intro.
+  - constructor. assumption.
+  - rewrite H. constructor. assumption.
+  - econstructor; try eassumption.
+    + apply IHtyping1; try assumption.
+    + apply IHtyping2; try assumption.
+      * intro. unfold lift at 2 3. destruct (lt_dec (proj1_sig i) n); simpl.
+        -- rewrite ren_comp. destruct (lt_dec _ _); try tauto.
+           epose proof (proj2_sig (σ (exist _ (proj1_sig i) l))). simpl in *.
+           destruct (lt_dec _ _); try tauto.
+           replace l1 with (proj2_sig (σ (exist _ (proj1_sig i) l))) by apply le_unique.
+           rewrite <- H. rewrite ren_comp. simpl. replace l with l0 by apply le_unique.
+           apply ren_ext, lift_weaken.
+        -- destruct (lt_dec _ _); try tauto. rewrite ren_comp. destruct (lt_dec _ _); try lia.
+           rewrite ren_comp. apply ren_ext, lift_weaken.
+      * econstructor; try assumption. apply IHtyping1; assumption.
+  - econstructor; try eassumption.
+    + apply IHtyping1; assumption.
+    + apply IHtyping2.
+      * intro. unfold lift at 2 3. destruct (lt_dec (proj1_sig i) n); simpl.
+        -- rewrite ren_comp. destruct (lt_dec _ _); try tauto.
+           epose proof (proj2_sig (σ (exist _ (proj1_sig i) l))). simpl in *.
+           destruct (lt_dec _ _); try tauto.
+           replace l1 with (proj2_sig (σ (exist _ (proj1_sig i) l))) by apply le_unique.
+           rewrite <- H. rewrite ren_comp. simpl. replace l with l0 by apply le_unique.
+           apply ren_ext, lift_weaken.
+        -- destruct (lt_dec _ _); try tauto. rewrite ren_comp. destruct (lt_dec _ _); try lia.
+           rewrite ren_comp. apply ren_ext, lift_weaken.
+      * econstructor; eauto.
+    + apply IHtyping3.
+      * intro. unfold lift at 2 3. destruct (lt_dec (proj1_sig i) n); simpl.
+        -- rewrite ren_comp. destruct (lt_dec _ _); try tauto.
+           epose proof (proj2_sig (σ (exist _ (proj1_sig i) l))). simpl in *.
+           destruct (lt_dec _ _); try tauto.
+           replace l1 with (proj2_sig (σ (exist _ (proj1_sig i) l))) by apply le_unique.
+           rewrite <- H. rewrite ren_comp. simpl. replace l with l0 by apply le_unique.
+           apply ren_ext, lift_weaken.
+        -- destruct (lt_dec _ _); try tauto. rewrite ren_comp. destruct (lt_dec _ _); try lia.
+           rewrite ren_comp. apply ren_ext, lift_weaken.
+      * econstructor; eauto.
+  - simpl in *. rewrite ren_bind.
+    replace (bind (ren σ ∘ bind_first u) B) with (bind (bind_first (ren σ u)) (ren (lift σ) B)).
+    + econstructor; eauto.
+    + rewrite bind_ren. apply bind_ext. intro. unfold lift, bind_first. simpl.
+      destruct (lt_dec _ n).
+      * simpl. pose proof (proj2_sig (σ (exist _ (proj1_sig i) l))). simpl in *.
+        destruct (lt_dec _ _); try tauto. f_equal. apply sig_lt_ext. reflexivity.
+      * simpl. destruct (lt_dec _ _); try lia. reflexivity.
+  - econstructor.
+    + apply IHtyping; assumption.
+    + apply ren_preserves_step_equiv. assumption.
+Qed.
+
+Lemma preservation (Sc: pi_scheme) {n} Γ (t u : term n) A :
+  Γ ⊢(Sc) t : A -> t ≻ u -> Γ ⊢(Sc) u : A.
+Proof.
+  induction 1; intro red; inversion red; clear red;
+    match goal with H : fill ?K _ = _ _ |- _ => (destruct K; simpl in *; try discriminate;
+    subst; try solve [ match goal with H : _ [≻] _ |- _ => inversion H end ]) | _ => idtac end.
+  - inversion H2; subst; clear H2. econstructor; try eassumption.
+    + apply IHtyping1. constructor. assumption.
+    + eapply equiv_context; try eassumption.
+      * simpl. intros. destruct (lt_dec _ _); try solve [constructor].
+        apply ren_preserves_step_equiv. apply Requiv_clot_r. constructor. assumption.
+      * econstructor; try eauto. { eapply typing_imp_ctx_wf. eassumption. } apply IHtyping1.
+        constructor. assumption.
+  - inversion H2; subst; clear H2. econstructor; try eassumption.
+    apply IHtyping2. constructor. assumption.
+  - inversion H3; subst; clear H3. unshelve econstructor. { exact (Pi (fill K u0) B). }
+    + econstructor; try eauto.
+      * apply IHtyping1. constructor. assumption.
+      * eapply equiv_context; try eassumption.
+        -- simpl. intros. destruct (lt_dec _ _); try solve [constructor].
+           apply ren_preserves_step_equiv, Requiv_clot_r. constructor. assumption.
+        -- econstructor.
+           ++ eapply typing_imp_ctx_wf; eassumption.
+           ++ apply IHtyping1. constructor. assumption.
+      * eapply equiv_context; try eassumption.
+        -- simpl. intros. destruct (lt_dec _ _); try solve [constructor].
+           apply ren_preserves_step_equiv, Requiv_clot_r. constructor. assumption.
+        -- econstructor.
+           ++ eapply typing_imp_ctx_wf; eassumption.
+           ++ apply IHtyping1. constructor. assumption.
+    + apply Requiv_clot_r. change (Pi (fill K ?x) B) with (fill (PiL K B) x). constructor.
+      assumption.
+  - inversion H3; subst; clear H3. econstructor; try eassumption.
+    apply IHtyping3. constructor. assumption.
+  - inversion H2; subst; clear H2. clear IHtyping1 IHtyping2.
+    rename u0 into u.
+    apply typ_abs_inv in H. destruct H as [s [s' [B0 H]]].
+    destruct H as [Hequiv [type_ty [type_B0 [type_body pi_check]]]].
+    apply pi_equiv_pi in Hequiv as [Aequiv Bequiv].
+    assert (true_type_body : Γ, ty ⊢(Sc) body : B).
+    { econstructor; eauto using Requiv_sym. }
+    assert (true_type_u : Γ ⊢(Sc) u : ty).
+    { econstructor; eauto. }
+    revert true_type_body true_type_u. clear. intros tybody tyu.
+    enough (
+        forall n k (σ : {i | i < k} -> term n) Γ Γ' x T,
+          (forall i, Γ ⊢(Sc) σ i : bind σ (kth_index_ctx Γ' (proj1_sig i) (proj2_sig i))) ->
+          Γ' ⊢(Sc) x : T -> Γ ⊢(Sc) -> Γ ⊢(Sc) bind σ x : bind σ T).
+    { eapply H; eauto using typing_imp_ctx_wf.
+      intro. destruct i; simpl. unfold bind_first at 1. simpl. destruct (lt_dec _ _).
+      - rewrite bind_ren. rewrite bind_id.
+        + constructor. eapply typing_imp_ctx_wf; eassumption.
+        + unfold bind_first, weaken. simpl. intro. pose proof (proj2_sig k). simpl in *.
+          destruct (lt_dec _ _); try tauto. f_equal. apply sig_lt_ext. reflexivity.
+      - rewrite bind_ren. rewrite bind_id; try assumption.
+        unfold bind_first, weaken. simpl. intro. pose proof (proj2_sig k). simpl in *.
+        destruct (lt_dec _ _); try tauto. f_equal. apply sig_lt_ext. reflexivity.
+    }
+    clear. intros ? ? ? ? ? ? ? H tyx Γwf. induction tyx in n, σ, Γ, H, Γwf |- *; simpl in *; auto.
+    + constructor. assumption.
+    + econstructor; eauto. eapply IHtyx2.
+      * intro. unfold lift_bind at 1. destruct (lt_dec _ _).
+        -- rewrite bind_weaken. eapply weakening.
+           ++ intro. simpl. pose proof (proj2_sig i0). destruct (lt_dec _ _); try tauto.
+              f_equal. f_equal. apply le_unique.
+           ++ apply H.
+           ++ econstructor; eauto.
+        -- rewrite bind_weaken.
+           replace (ren weaken (bind σ A)) with
+             (kth_index_ctx (Γ, bind σ A) n (Nat.lt_succ_diag_r n)).
+           ++ constructor. econstructor; eauto.
+           ++ simpl. destruct (lt_dec n n); try lia. reflexivity.
+      * econstructor; eauto.
+    + econstructor; eauto.
+      * apply IHtyx2.
+        -- intro. rewrite bind_weaken. unfold lift_bind.
+           destruct (lt_dec _ _).
+           ++ eapply weakening; eauto.
+              ** intro. simpl. pose proof (proj2_sig i0). simpl in *.
+                 destruct (lt_dec _ _); try tauto. f_equal. f_equal. apply le_unique.
+              ** econstructor; eauto.
+           ++ replace (ren weaken (bind σ A)) with
+                (kth_index_ctx (Γ, bind σ A) n (Nat.lt_succ_diag_r n)).
+              ** do 2 econstructor; eauto.
+              ** simpl. destruct (lt_dec _ _); try lia. reflexivity.
+        -- econstructor; eauto.
+      * apply IHtyx3.
+        -- intro. rewrite bind_weaken. unfold lift_bind at 1. destruct (lt_dec _ _).
+           ++ eapply weakening; eauto.
+              ** intro. simpl. pose proof (proj2_sig i0). simpl in *.
+                 destruct (lt_dec _ _); try tauto. f_equal. f_equal. apply le_unique.
+              ** econstructor; eauto.
+           ++ replace (ren weaken (bind σ A)) with
+                (kth_index_ctx (Γ, bind σ A) n (Nat.lt_succ_diag_r n)).
+              ** do 2 econstructor; eauto.
+              ** simpl. destruct (lt_dec _ _); try lia. reflexivity.
+        -- econstructor; eauto.
+    + rewrite bind_comp. replace (bind (bind σ ∘ bind_first u) B) with
+        (bind (bind_first (bind σ u)) (bind (lift_bind σ) B)).
+      * econstructor; eauto.
+      * rewrite bind_comp. apply bind_ext. intro. unfold lift_bind, bind_first at 2.
+        destruct (lt_dec _ _); simpl.
+        -- rewrite bind_ren. apply bind_id. intro. unfold weaken, bind_first. simpl.
+           pose proof (proj2_sig k). simpl in *. destruct (lt_dec _ _); try tauto.
+           f_equal. apply sig_lt_ext. reflexivity.
+        -- unfold bind_first. simpl. destruct (lt_dec _ _); try lia. reflexivity.
+    + econstructor; eauto. apply bind_preserves_step_equiv. assumption.
+  - inversion H1; subst; clear H1. econstructor; try eassumption.
+    apply IHtyping1. constructor. assumption.
+  - inversion H1; subst; clear H1. econstructor.
+    + econstructor; try eassumption. apply IHtyping2. constructor. assumption.
+    + apply bind_preserves_step_equiv_in_subs. intro. unfold bind_first.
+      destruct (lt_dec _ _).
+      * constructor.
+      * apply Requiv_clot_r. constructor. assumption.
+  - subst. econstructor; try eassumption. apply IHtyping. constructor. assumption.
+Qed.
